src/program_logic/private_invariants.v
@@ -235,4 +235,45 @@ Context `{PRI: !pri_invG IRISG}.
   Global Instance pri_inv_persistent E P : Persistent (pri_inv E P).
   Proof. rewrite pri_inv_eq. apply _. Qed.
 
+  Lemma wpc0_pri_inv_tok_res s k mj E1 e Φ Φc :
+    (∀ D E', pri_inv_tok 1%Qp E' ∗ ⌜ (/2 < mj)%Qp ∧ E' ## D ⌝ -∗ ||={E1|⊤∖D, E1|⊤∖D}=> wpc0 s k mj E1 e Φ Φc) -∗
+    wpc0 s k mj E1 e Φ Φc.
+  Proof.
+    iIntros "H".
+    iEval (rewrite wpc0_unfold).
+    rewrite /wpc_pre.
+    iSplit.
+    {
+      destruct (to_val e) eqn:Heq_val.
+      - iIntros (q g1 ns D κs) "Hg HNC".
+        iMod (pri_inv_tok_alloc with "[$]") as (Einv Hdisj) "(Hitok&Hg)".
+        iDestruct (pri_inv_tok_global_valid with "[$]") as %(?&?).
+        iSpecialize ("H" with "[$Hitok //]").
+        rewrite wpc0_unfold/ wpc_pre. rewrite Heq_val.
+        iMod "H" as "(H&_)". by iMod ("H" with "[$] [$]") as "$".
+      - iIntros.
+        iMod (pri_inv_tok_alloc with "[$]") as (Einv Hdisj) "(Hitok&Hg)".
+        iDestruct (pri_inv_tok_global_valid with "[$]") as %(?&?).
+        iSpecialize ("H" with "[$Hitok //]").
+        rewrite wpc0_unfold/ wpc_pre. rewrite Heq_val.
+        iMod "H" as "(H&_)". by iMod ("H" with "[$] [$] [$]") as "$".
+    }
+    iIntros.
+    iMod (pri_inv_tok_alloc with "[$]") as (Einv Hdisj) "(Hitok&Hg)".
+    iDestruct (pri_inv_tok_global_valid with "[$]") as %(?&?).
+    iSpecialize ("H" with "[$Hitok //]").
+    rewrite wpc0_unfold/ wpc_pre.
+    iMod "H" as "(_&H)". by iMod ("H" with "[$] [$]") as "$".
+  Qed.
+
+  Lemma wpc_pri_inv_tok_res s k E1 e Φ Φc :
+    (∀ E', pri_inv_tok 1%Qp E' -∗ wpc s k E1 e Φ Φc) -∗
+    wpc s k E1 e Φ Φc.
+  Proof.
+    iIntros "H". rewrite wpc_eq. iIntros (mj).
+    iApply wpc0_pri_inv_tok_res. iIntros (D E') "(Htok&%)".
+    iModIntro. iSpecialize ("H" with "[$]"). iSpecialize ("H" $! mj).
+    eauto.
+  Qed.
+
 End pri_inv.
